Foundation/Propositional/Kripke/Logic/Cl.lean
@@ -13,7 +13,7 @@ namespace Kripke
 
 variable {F : Frame}
 
-protected abbrev Frame.IsCl := Frame.IsEuclidean
+@[reducible] protected alias Frame.IsCl := Frame.IsEuclidean
 protected class Frame.IsFiniteCl (F : Frame) extends F.IsFinite, F.IsCl
 
 instance : whitepoint.IsEuclidean := ⟨by tauto⟩
@@ -36,30 +36,30 @@ namespace Hilbert
 
 namespace Cl.Kripke
 
-instance sound : Sound Hilbert.Cl FrameClass.Cl :=
+instance : Sound Hilbert.Cl FrameClass.Cl :=
   instSound_of_validates_axioms $ by
     apply FrameClass.Validates.withAxiomEFQ;
     rintro F hF _ rfl;
     replace hF := Set.mem_setOf_eq.mp hF;
     apply validate_axiomLEM_of_isEuclidean;
 
-instance sound_finite : Sound Hilbert.Cl FrameClass.finite_Cl :=
+instance : Sound Hilbert.Cl FrameClass.finite_Cl :=
   instSound_of_validates_axioms $ by
     apply FrameClass.Validates.withAxiomEFQ;
     rintro F ⟨_, hF⟩ _ rfl;
     apply validate_axiomLEM_of_isEuclidean;
 
-instance consistent : Entailment.Consistent Hilbert.Cl := consistent_of_sound_frameclass FrameClass.Cl $ by
+instance : Entailment.Consistent Hilbert.Cl := consistent_of_sound_frameclass FrameClass.Cl $ by
   use whitepoint;
   apply Set.mem_setOf_eq.mpr;
   infer_instance
 
-instance canonical : Canonical Hilbert.Cl FrameClass.Cl :=  ⟨by
+instance : Canonical Hilbert.Cl FrameClass.Cl :=  ⟨by
   apply Set.mem_setOf_eq.mpr;
   infer_instance;
 ⟩
 
-instance complete : Complete Hilbert.Cl FrameClass.Cl := inferInstance
+instance : Complete Hilbert.Cl FrameClass.Cl := inferInstance
 
 section FFP
 
@@ -67,7 +67,7 @@ open
   finestFiltrationTransitiveClosureModel
   Relation
 
-instance complete_finite_symmetric : Complete Hilbert.Cl FrameClass.finite_Cl := by
+instance : Complete Hilbert.Cl FrameClass.finite_Cl := by
   suffices Complete Hilbert.Cl { F : Frame | F.IsFinite ∧ F.IsSymmetric } by
     convert this;
     constructor;
@@ -76,7 +76,7 @@ instance complete_finite_symmetric : Complete Hilbert.Cl FrameClass.finite_Cl :=
 
   constructor;
   intro φ hφ;
-  apply Kripke.complete.complete;
+  apply Complete.complete (𝓜 := FrameClass.Cl);
   rintro F F_con V r;
   replace F_con := Set.mem_setOf_eq.mp F_con;
   let M : Kripke.Model := ⟨F, V⟩;
@@ -114,6 +114,8 @@ instance complete_finite_symmetric : Complete Hilbert.Cl FrameClass.finite_Cl :=
 
 end FFP
 
+end Cl.Kripke
+
 instance : Hilbert.LC ⪱ Hilbert.Cl := by
   constructor;
   . apply Hilbert.weakerThan_of_provable_axioms;
@@ -141,8 +143,6 @@ instance : Hilbert.LC ⪱ Hilbert.Cl := by
         have := @F.eucl _ 0 1 0;
         omega;
 
-end Cl.Kripke
-
 instance : Hilbert.Int ⪱ Hilbert.Cl := calc
   Hilbert.Int ⪱ Hilbert.KC := inferInstance
   _           ⪱ Hilbert.LC := inferInstance
@@ -150,15 +150,10 @@ instance : Hilbert.Int ⪱ Hilbert.Cl := calc
 
 end Hilbert
 
+propositional_kripke Logic.Cl FrameClass.Cl
+propositional_kripke Logic.Cl FrameClass.finite_Cl
 
-namespace Logic
-
-lemma Cl.Kripke.Cl : Logic.Cl = FrameClass.Cl.logic := eq_Hilbert_Logic_KripkeFrameClass_Logic
-lemma Cl.Kripke.finite_Cl : Logic.Cl = FrameClass.finite_Cl.logic := eq_Hilbert_Logic_KripkeFrameClass_Logic
-
+instance : Logic.LC ⪱ Logic.Cl := inferInstance
 instance : Logic.Int ⪱ Logic.Cl := inferInstance
-
-end Logic
-
 
 end LO.Propositional
