Foundation/Propositional/Kripke/Logic/LC.lean
@@ -10,7 +10,8 @@ open Formula.Kripke
 namespace Kripke
 
 variable {F : Frame}
-protected abbrev Frame.IsLC := Frame.IsPiecewiseStronglyConnected
+
+@[reducible] protected alias Frame.IsLC := Frame.IsPiecewiseStronglyConnected
 protected class Frame.IsFiniteLC (F : Frame) extends F.IsFinite, F.IsLC
 
 protected abbrev FrameClass.LC : FrameClass := { F | F.IsLC }
@@ -19,42 +20,38 @@ protected abbrev FrameClass.finite_LC : FrameClass := { F | F.IsFiniteLC }
 end Kripke
 
 
-namespace Hilbert.LC.Kripke
+namespace Hilbert
 
-instance sound : Sound Hilbert.LC FrameClass.LC := instSound_of_validates_axioms $ by
-    apply FrameClass.Validates.withAxiomEFQ;
-    rintro F hF _ rfl;
-    replace hF := Set.mem_setOf_eq.mp hF;
-    apply validate_axiomDummett_of_isPiecewiseStronglyConnected;
+namespace LC.Kripke
 
-instance sound_finite : Sound Hilbert.LC FrameClass.finite_LC :=
-  instSound_of_validates_axioms $ by
-    apply FrameClass.Validates.withAxiomEFQ;
-    rintro F hF _ rfl;
-    replace hF := Set.mem_setOf_eq.mp hF;
-    apply validate_axiomDummett_of_isPiecewiseStronglyConnected;
+instance : Sound Hilbert.LC FrameClass.LC := instSound_of_validates_axioms $ by
+  apply FrameClass.Validates.withAxiomEFQ;
+  rintro F hF _ rfl;
+  replace hF := Set.mem_setOf_eq.mp hF;
+  apply validate_axiomDummett_of_isPiecewiseStronglyConnected;
 
-instance consistent : Entailment.Consistent Hilbert.LC := consistent_of_sound_frameclass FrameClass.LC $ by
+instance : Sound Hilbert.LC FrameClass.finite_LC := instSound_of_validates_axioms $ by
+  apply FrameClass.Validates.withAxiomEFQ;
+  rintro F hF _ rfl;
+  replace hF := Set.mem_setOf_eq.mp hF;
+  apply validate_axiomDummett_of_isPiecewiseStronglyConnected;
+
+instance : Entailment.Consistent Hilbert.LC := consistent_of_sound_frameclass FrameClass.LC $ by
   use whitepoint;
   apply Set.mem_setOf_eq.mpr;
   infer_instance
 
-instance canonical : Canonical Hilbert.LC FrameClass.LC := ⟨by
+instance : Canonical Hilbert.LC FrameClass.LC := ⟨by
   apply Set.mem_setOf_eq.mpr;
   infer_instance;
 ⟩
 
-instance complete : Complete Hilbert.LC FrameClass.LC := inferInstance
+instance : Complete Hilbert.LC FrameClass.LC := inferInstance
 
-section FFP
-
-open
-  finestFiltrationTransitiveClosureModel
-  Relation
-
-instance finite_complete : Complete Hilbert.LC FrameClass.finite_LC := ⟨by
+open finestFiltrationTransitiveClosureModel Relation in
+instance : Complete Hilbert.LC FrameClass.finite_LC := ⟨by
   intro φ hφ;
-  apply Kripke.complete.complete;
+  apply Complete.complete (𝓜 := FrameClass.LC);
   rintro F F_conn V r;
   replace F_conn := Set.mem_setOf_eq.mp F_conn;
   let M : Kripke.Model := ⟨F, V⟩;
@@ -100,10 +97,9 @@ instance finite_complete : Complete Hilbert.LC FrameClass.finite_LC := ⟨by
           use Z, Y;
           tauto;
   }
-
 ⟩
 
-end FFP
+end LC.Kripke
 
 instance : Hilbert.KC ⪱ Hilbert.LC := by
   constructor;
@@ -137,16 +133,13 @@ instance : Hilbert.KC ⪱ Hilbert.LC := by
         by_contra hC;
         simpa using @hC.ps_connected 0 1 2;
 
-end Hilbert.LC.Kripke
+end Hilbert
 
 
-namespace Logic
-
-lemma LC.Kripke.LC : Logic.LC = FrameClass.LC.logic := eq_Hilbert_Logic_KripkeFrameClass_Logic
-lemma LC.Kripke.finite_LC : Logic.LC = FrameClass.finite_LC.logic := eq_Hilbert_Logic_KripkeFrameClass_Logic
+propositional_kripke Logic.LC FrameClass.LC
+propositional_kripke Logic.LC FrameClass.finite_LC
 
 instance : Logic.KC ⪱ Logic.LC := inferInstance
 
-end Logic
 
 end LO.Propositional
