Foundation/Propositional/ClassicalSemantics/Hilbert.lean
@@ -115,7 +115,7 @@ end Completeness
 end Hilbert.Cl
 
 
-namespace Cl
+namespace Logic.Cl
 
 variable {φ : Formula ℕ}
 
@@ -123,6 +123,12 @@ theorem tautologies : Logic.Cl = { φ | φ.isTautology } := by
   ext φ;
   simp [Hilbert.Cl.iff_isTautology_provable, Entailment.theory];
 
-end Cl
+lemma exists_valuation_of_not (h : Logic.Cl ⊬ φ) : ∃ v : Valuation _, ¬(v ⊧ φ) := by
+  apply Hilbert.Cl.exists_valuation_of_not_provable;
+  tauto;
+
+lemma iff_isTautology : Logic.Cl ⊢! φ ↔ φ.isTautology := by simp [tautologies];
+
+end Logic.Cl
 
 end LO.Propositional
